chore

Auto/Lib/Pos.lean
@@ -13,24 +13,26 @@ namespace Pos
 
 abbrev one := xH
 
-def toNat : Pos → Nat
+def toNat' : Pos → Nat
 | xH => 1
-| xO p' => p'.toNat * 2
-| xI p' => p'.toNat * 2 + 1
+| xO p' => p'.toNat' * 2
+| xI p' => p'.toNat' * 2 + 1
 
-theorem toNat_not_zero (p : Pos) : toNat p ≠ 0 := by
+def toNat (p : Pos) := Nat.pred (toNat' p)
+
+theorem toNat'_not_zero (p : Pos) : toNat' p ≠ 0 := by
   induction p
   case xH => intro H; contradiction
   case xO p' IH =>
-    simp [toNat]; intro H
+    simp [toNat']; intro H
     rw [Nat.mul_eq_zero] at H
     cases H
     case inl H' => revert H'; exact IH
     case inr H' => cases H'
   case xI p' _ =>
-    simp [toNat] 
+    simp [toNat'] 
 
-private theorem ofNatWFAux (n n' : Nat) : n = n' + 2 → n / 2 < n := by
+private theorem ofNat'WFAux (n n' : Nat) : n = n' + 2 → n / 2 < n := by
   intro H; apply Nat.div_lt_self
   case hLtN =>
     cases n;
@@ -38,17 +40,17 @@ private theorem ofNatWFAux (n n' : Nat) : n = n' + 2 → n / 2 < n := by
     apply Nat.succ_le_succ; apply Nat.zero_le
   case hLtK => apply Nat.le_refl
 
-def ofNatWF (n : Nat) :=
+def ofNat'WF (n : Nat) :=
   match h : n with
   | 0 => xH
   | 1 => xH
   | _ + 2 =>
     match n % 2 with
-    | 0 => .xO (ofNatWF (n / 2))
-    | _ => .xI (ofNatWF (n / 2))
-decreasing_by apply ofNatWFAux; assumption
+    | 0 => .xO (ofNat'WF (n / 2))
+    | _ => .xI (ofNat'WF (n / 2))
+decreasing_by apply ofNat'WFAux; assumption
 
-theorem ofNatWF.inductionOn.{u}
+theorem ofNat'WF.inductionOn.{u}
   {motive : Nat → Sort u} (x : Nat)
   (ind : ∀ x, motive ((x + 2) / 2) → motive (x + 2))
   (base₀ : motive 0) (base₁ : motive 1) : motive x :=
@@ -56,42 +58,42 @@ theorem ofNatWF.inductionOn.{u}
   | 0 => base₀
   | 1 => base₁
   | x' + 2 => ind x' (inductionOn ((x' + 2) / 2) ind base₀ base₁)
-decreasing_by apply ofNatWFAux; rfl
+decreasing_by apply ofNat'WFAux; rfl
 
-theorem ofNatWF.induction
+theorem ofNat'WF.induction
   {motive : Nat → Sort u}
   (ind : ∀ x, motive ((x + 2) / 2) → motive (x + 2))
   (base₀ : motive 0) (base₁ : motive 1) : ∀ x, motive x :=
-  fun x => ofNatWF.inductionOn x ind base₀ base₁
+  fun x => ofNat'WF.inductionOn x ind base₀ base₁
 
-theorem ofNatWF.succSucc (n : Nat) :
-  ofNatWF (n + 2) =
+theorem ofNat'WF.succSucc (n : Nat) :
+  ofNat'WF (n + 2) =
     match (n + 2) % 2 with
-    | 0 => .xO (ofNatWF ((n + 2) / 2))
-    | _ => .xI (ofNatWF ((n + 2) / 2)) := rfl
+    | 0 => .xO (ofNat'WF ((n + 2) / 2))
+    | _ => .xI (ofNat'WF ((n + 2) / 2)) := rfl
 
-theorem ofNatWF.double_xO (n : Nat) :
-  n ≠ 0 → ofNatWF (n * 2) = xO (ofNatWF n) :=
+theorem ofNat'WF.double_xO (n : Nat) :
+  n ≠ 0 → ofNat'WF (n * 2) = xO (ofNat'WF n) :=
   match n with
   | 0 => by intro H; contradiction
-  | 1 => fun _ => by simp [ofNatWF]
+  | 1 => fun _ => by simp [ofNat'WF]
   | n' + 2 => fun _ => by
     rw [Nat.mul_comm, Nat.mul_add];
-    rw [ofNatWF.succSucc];
+    rw [ofNat'WF.succSucc];
     have heq : (2 * n' + 2 + 2) % 2 = 0 := by
       rw [Nat.add_mod_right]; rw [Nat.add_mod_right]
       rw [Nat.mul_mod]; simp
     rw [heq]; simp
 
-theorem ofNatWF.doubleSucc_xI (n : Nat) :
-  n ≠ 0 → ofNatWF ((n * 2) + 1) = xI (ofNatWF n) :=
+theorem ofNat'WF.doubleSucc_xI (n : Nat) :
+  n ≠ 0 → ofNat'WF ((n * 2) + 1) = xI (ofNat'WF n) :=
   match n with
   | 0 => by intro H; contradiction
-  | 1 => fun _ => by simp [ofNatWF]
+  | 1 => fun _ => by simp [ofNat'WF]
   | n' + 2 => fun _ => by
     rw [Nat.mul_comm, Nat.mul_add];
     have : (2 * n' + 2 * 2 + 1) = (2 * n') + 3 + 2 := rfl
-    rw [ofNatWF.succSucc];
+    rw [ofNat'WF.succSucc];
     have heq : (2 * n' + 3 + 2) % 2 = 1 := by
       rw [Nat.add_mod_right]; rw [Nat.add_mod]
       rw [Nat.mul_mod]; simp
@@ -101,20 +103,20 @@ theorem ofNatWF.doubleSucc_xI (n : Nat) :
       rw [Nat.add_mul_div_left _ _ (by simp)]; rw [Nat.add_comm]; rfl;
     rw [heq']
 
-theorem ofNatWF_toNat (p : Pos) : ofNatWF (toNat p) = p := by
+theorem ofNat'WF_toNat' (p : Pos) : ofNat'WF (toNat' p) = p := by
   induction p
   case xH => rfl
   case xO p' IH =>
-    dsimp [toNat];
-    rw [ofNatWF.double_xO];
-    rw [IH]; apply toNat_not_zero
+    dsimp [toNat'];
+    rw [ofNat'WF.double_xO];
+    rw [IH]; apply toNat'_not_zero
   case xI p' IH =>
-    dsimp [toNat];
-    rw [ofNatWF.doubleSucc_xI];
-    rw [IH]; apply toNat_not_zero
+    dsimp [toNat'];
+    rw [ofNat'WF.doubleSucc_xI];
+    rw [IH]; apply toNat'_not_zero
 
-theorem toNat_ofNatWF (n : Nat) : n ≠ 0 → toNat (ofNatWF n) = n := by
-  revert n; apply ofNatWF.induction
+theorem toNat'_ofNat'WF (n : Nat) : n ≠ 0 → toNat' (ofNat'WF n) = n := by
+  revert n; apply ofNat'WF.induction
   case base₀ => intro H; contradiction
   case base₁ => intro H; rfl
   case ind =>
@@ -122,16 +124,16 @@ theorem toNat_ofNatWF (n : Nat) : n ≠ 0 → toNat (ofNatWF n) = n := by
     have hne : (x + 2) / 2 ≠ 0 := by
       rw [Nat.add_div_right]; simp; simp
     have IH' := IH hne
-    rw [ofNatWF.succSucc];
+    rw [ofNat'WF.succSucc];
     have heq : (x + 2) / 2 = Nat.succ (x / 2) := Nat.add_div_right _ (by simp)
     rw [heq] at IH'
     match h : (x + 2) % 2 with
     | 0 =>
-      simp [toNat]; rw [IH'];
+      simp [toNat']; rw [IH'];
       rw [← Nat.mod_add_div (x + 2) 2];
       rw [h]; simp; apply Nat.mul_comm
     | 1 =>
-      simp [toNat]; rw [IH'];
+      simp [toNat']; rw [IH'];
       rw [Nat.add_mul _ 1]; simp
       calc
         _ = 2 * (x / 2) + x % 2 := by
@@ -145,7 +147,7 @@ theorem toNat_ofNatWF (n : Nat) : n ≠ 0 → toNat (ofNatWF n) = n := by
       apply Nat.mod_lt; simp
       apply Nat.succ_le_succ; apply Nat.succ_le_succ; apply Nat.zero_le
 
-def ofNatRD (rd : Nat) (n : Nat) :=
+def ofNat'RD (rd : Nat) (n : Nat) :=
   match rd with
   | 0 => xH
   | .succ rd' =>
@@ -154,21 +156,21 @@ def ofNatRD (rd : Nat) (n : Nat) :=
     | 1 => xH
     | _ =>
       match Nat.mod n 2 with
-      | 0 => .xO (ofNatRD rd' (Nat.div n 2))
-      | _ => .xI (ofNatRD rd' (Nat.div n 2))
+      | 0 => .xO (ofNat'RD rd' (Nat.div n 2))
+      | _ => .xI (ofNat'RD rd' (Nat.div n 2))
 
-theorem ofNat.equivAux (rd n : Nat) : rd ≥ n → ofNatWF n = ofNatRD rd n := by
+theorem ofNat'.equivAux (rd n : Nat) : rd ≥ n → ofNat'WF n = ofNat'RD rd n := by
   revert n; induction rd <;> intros n H
   case zero =>
     have hzero : n = 0 := Nat.eq_zero_of_le_zero H
     rw [hzero]; rfl
   case succ rd' IH =>
-    dsimp [ofNatRD]
+    dsimp [ofNat'RD]
     match n with
     | 0 => rfl
     | 1 => rfl
     | n' + 2 =>
-      rw [ofNatWF.succSucc]; simp;
+      rw [ofNat'WF.succSucc]; simp;
       have heq' : Nat.mod (n' + 2) 2 = n' % 2 := by
         suffices (n' + 2) % 2 = n' % 2 by exact this
         rw [Nat.add_mod_right]
@@ -180,10 +182,12 @@ theorem ofNat.equivAux (rd n : Nat) : rd ≥ n → ofNatWF n = ofNatRD rd n := b
       case a.a => apply Nat.succ_le_succ; apply Nat.div_le_self
       case a.a => apply Nat.le_of_succ_le_succ H
 
-def ofNat n := ofNatRD n n
+def ofNat' n := ofNat'RD n n
 
-theorem ofNat.equiv (n : Nat) : ofNatWF n = ofNat n :=
-  ofNat.equivAux n n (Nat.le_refl _)
+theorem ofNat'.equiv (n : Nat) : ofNat'WF n = ofNat' n :=
+  ofNat'.equivAux n n (Nat.le_refl _)
+
+def ofNat n := ofNat' (.succ n)
 
 def reprPrec (p : Pos) (_ : Nat) : Lean.Format :=
   f!"Pos.ofNat {p.toNat}"
